implement Close

Hyper.dfy
@@ -2,11 +2,13 @@
 
 type Pid = int
 type FD = int
-type RefCount = int
+type RefCount = nat
 type FileTableEntry = int
 
+datatype File = File(in_use: bool, refcount: RefCount)
+
 class State {
-    var file_table: array<RefCount>
+    var file_table: array<File>
     var proc_fd_tables: map<Pid, array<FileTableEntry>>
 
     ghost var repr: set<object>
@@ -36,14 +38,14 @@ class State {
         reads this, repr
     {
         && ReprValid()
-        && (forall proc | proc in proc_fd_tables ::
-            && (forall fd | 0 <= fd < proc_fd_tables[proc].Length ::
-                var f := proc_fd_tables[proc][fd];
-                f == -1 || 0 <= f < file_table.Length))
+        && (forall proc, fd | proc in proc_fd_tables && 0 <= fd < proc_fd_tables[proc].Length ::
+            var f := proc_fd_tables[proc][fd];
+            f == -1 || (0 <= f < file_table.Length && file_table[f].in_use))
         && (forall p1, p2 | p1 in proc_fd_tables && p2 in proc_fd_tables && p1 != p2 ::
             proc_fd_tables[p1] != proc_fd_tables[p2])
-        && (forall proc | proc in proc_fd_tables :: proc_fd_tables[proc] != file_table)
-        && (forall f | 0 <= f < file_table.Length :: file_table[f] == |References(f)|)
+        && (forall f | 0 <= f < file_table.Length ::
+            && file_table[f].refcount == |References(f)|
+            && (file_table[f].in_use <==> file_table[f].refcount > 0))
     }
 }
 
@@ -80,10 +82,10 @@ method Dup(s: State, proc: Pid, oldfd: FD) returns (ok: bool, newfd: FD)
     assert oldfd != newfd;
     var f := fd_table[oldfd];
     fd_table[newfd] := f;
-    s.file_table[f] := s.file_table[f] + 1;
+    s.file_table[f] := s.file_table[f].(refcount := s.file_table[f].refcount + 1);
 
-    forall f' | 0 <= f' < s.file_table.Length
-        ensures s.file_table[f'] == |s.References(f')|
+    forall f' | 0 <= f' < s.file_table.Length && s.file_table[f'].in_use
+        ensures s.file_table[f'].refcount == |s.References(f')|
     {
         if f == f' {
             assert s.References(f) == old(s.References(f)) + {(proc, newfd)};
@@ -117,10 +119,10 @@ method DupFinite(s: State, proc: Pid, oldfd: FD, newfd: FD) returns (ok: bool)
     assert oldfd != newfd;
     var f := fd_table[oldfd];
     fd_table[newfd] := f;
-    s.file_table[f] := s.file_table[f] + 1;
+    s.file_table[f] := s.file_table[f].(refcount := s.file_table[f].refcount + 1);
 
-    forall f' | 0 <= f' < s.file_table.Length
-        ensures s.file_table[f'] == |s.References(f')|
+    forall f' | 0 <= f' < s.file_table.Length && s.file_table[f'].in_use
+        ensures s.file_table[f'].refcount == |s.References(f')|
     {
         if f == f' {
             assert s.References(f) == old(s.References(f)) + {(proc, newfd)};
@@ -130,4 +132,78 @@ method DupFinite(s: State, proc: Pid, oldfd: FD, newfd: FD) returns (ok: bool)
     }
 
     return true;
+}
+
+lemma CardinalitySubset<T>(A: set<T>, B: set<T>)
+    requires A <= B
+    ensures |A| <= |B|
+{
+    if A == B {
+        return;
+    } else {
+        assert A < B;
+        var x :| x in B && x !in A;
+        CardinalitySubset(A, B - {x});
+    }
+}
+
+lemma CardinalityOne<T>(S: set<T>, x: T)
+    requires |S| == 1 && x in S
+    ensures S == {x}
+{
+    forall y | y in S
+        ensures y == x
+    {
+        if y != x {
+            CardinalitySubset({x, y}, S);
+        }
+    }
+}
+
+lemma ValidReferences(s: State)
+    requires s != null && s.Valid()
+{}
+
+method Close(s: State, proc: Pid, fd: FD) returns (ok: bool)
+    requires s != null && s.Valid() && proc in s.proc_fd_tables
+    modifies s.repr
+    ensures s.Valid()
+    ensures s.proc_fd_tables == old(s.proc_fd_tables)
+    ensures forall proc' | proc' != proc && proc' in s.proc_fd_tables ::
+        s.proc_fd_tables[proc'][..] == old(s.proc_fd_tables[proc'][..])
+{
+    var fd_table := s.proc_fd_tables[proc];
+    if fd < 0 || fd >= fd_table.Length || fd_table[fd] == -1 { return false; }
+
+    var file := fd_table[fd];
+
+    if s.file_table[file].refcount == 1 {
+        assert forall proc', fd' |
+            && proc' in s.proc_fd_tables
+            && 0 <= fd' < s.proc_fd_tables[proc'].Length
+            :: (proc', fd') in s.References(file) || s.proc_fd_tables[proc'][fd'] != file;
+    
+        assert s.References(file) == {(proc, fd)} by {
+            CardinalityOne(s.References(file), (proc, fd));
+        }
+    }
+
+    fd_table[fd] := -1;
+
+    s.file_table[file] := s.file_table[file].(refcount := s.file_table[file].refcount - 1);
+
+    if s.file_table[file].refcount == 0 {
+        s.file_table[file] := s.file_table[file].(in_use := false);
+    }
+
+    forall f | 0 <= f < s.file_table.Length
+        ensures s.file_table[f].refcount == |s.References(f)|
+        ensures s.file_table[f].in_use <==> s.file_table[f].refcount > 0
+    {
+        if file == f {
+            assert s.References(file) == old(s.References(file)) - {(proc, fd)};
+        } else {
+            assert s.References(f) == old(s.References(f));
+        }
+    }
 }
